\documentclass[12pt]{article}
 \usepackage[margin=1in]{geometry} 
\usepackage{amsmath,amsthm,amssymb,amsfonts}
\usepackage{color}
\usepackage{mathtools, eucal}
\usepackage{xparse}
\usepackage{romannum}
 
\DeclarePairedDelimiter\floor{\lfloor}{\rfloor}
\newtheorem{theorem}{Theorem}[section]
\newtheorem{corollary}{Corollary}[theorem]
\newtheorem{lemma}[theorem]{Lemma}

 
\begin{document}
 
%\renewcommand{\qedsymbol}{\filledbox}
%Good resources for looking up how to do stuff:
%Binary operators: http://www.access2science.com/latex/Binary.html
%General help: http://en.wikibooks.org/wiki/LaTeX/Mathematics
%Or just google stuff
 
\title{MA 515 Homework 6}
\author{Zheming Gao}
\maketitle

\section*{Problem 1}

\begin{proof}

Given $\bar x \in X$, let $V = span \{\bar x\}$ and define linear bounded operator $F: V \rightarrow \mathbb R$, such that $\forall x \in V$, $F(x) = \|x\|$. Hence, by Hahn-Banach theorem, there exists $\Phi: X\rightarrow \mathbb R$ such that $\Phi = F$ on $V$ and $\|\Phi\|_\infty = \|F\|_\infty$. Since $\bar x \in V\subset X$, $\|\Phi(\bar x)\| =  \|F(\bar x)\| = \|\bar x\|$.

\end{proof}

\section*{Problem 2}

\begin{proof}

Suppose $x \neq y$. Let $V = span\{x, y\}$ functional $f: V\rightarrow \mathbb R $ such that $\forall s, t\in \mathbb R$, 

$$
f(sx + ty) = s\|x\| - t\|y\|.
$$

Hence, $f(x) = \|x\|$, $f(y) = -\|y\|$ and $f(x)\neq f(y)$. By the theorem, there exists a functional $F: X\rightarrow \mathbb R$ such that $F = f$ on $V$ and $\|f\|_\infty = \|F\|_\infty$, which is a contradiction.

\end{proof}

\section*{Problem 3}

\begin{proof}

Since $\Lambda: Y \rightarrow \mathbb R^n$, $\forall y\in Y$, $\Lambda(y) = (\Lambda_1(y), \dots, \Lambda_n(y))$, where linear bounded functionals $\Lambda_i : Y \rightarrow \mathbb R$, $\forall i = 1, \dots, n$. By Hahn-Banach theorem, there exists a linear bounded functional for each $i$ such that $\widetilde \Lambda_i: X \rightarrow \mathbb R$, and $\|\widetilde \Lambda_i\|_\infty = \|\Lambda_i\|_\infty$. Let operator $\widetilde\Lambda: X \rightarrow \mathbb R^n$ such that 

$$
\widetilde\Lambda(y) = (\widetilde\Lambda_1(y), \dots, \widetilde\Lambda_n(y)), \quad \forall y\in X.
$$

Also, we notice that $\|\Lambda_i\|_\infty \leqslant \|\Lambda\|_\infty$.
Then, $\forall x\in X\cap S(0, 1)$ 

$$
\begin{aligned}
\|\widetilde\Lambda(x)\| = & \sqrt{|\widetilde\Lambda_1(x)|^2 + \cdots + |\widetilde\Lambda_n(x)|^2} \\
 \leqslant & \sqrt{(\|\widetilde\Lambda_1\|_\infty^2 + \cdots + \|\widetilde\Lambda_n\|_\infty^2) \|x\|_X^2} \\
 = & \sqrt{(\|\Lambda_1\|_\infty^2 + \cdots + \|\Lambda_n\|_\infty^2)\|x\|_X^2} \\
 \leqslant & \sqrt{n} \|\Lambda\|_\infty \|x\|_X.
\end{aligned}
$$ 

Divided by $\|x\|_X$ on both sides and take supreme,we have

$$
\|\widetilde\Lambda\|_\infty \leqslant \sqrt{n} \|\Lambda\|_\infty.
$$

\end{proof}

\section*{Problem 4}

\begin{proof}

We apply Banach-Alaoglu theorem directly, so there exists a subsequence $\{\varphi_{n_k}\}$ such that $\varphi_{n_k} \overset{\ast}{\rightharpoonup} \varphi  $. Hence, for any $x\in X$, $\varphi_{n_k}(x) \rightarrow \varphi(x)$. Additionally, we know for any $y_k \in S$, $\varphi_{n}(y_k) \rightarrow \varphi(y_k)$ and $\overline S = X$. Hence, $\varphi_{n}(x) \rightarrow \varphi(x)$, $\forall x \in X$. And it is equivalent to $\varphi_{n} \overset{\ast}{\rightharpoonup} \varphi$ on $X$. 

Next, we need to show $\varphi$ is bounded. For any $x \in X\cap S(0, 1)$, 

$$ 
\|\varphi(x)\| = \lim_{n \rightarrow +\infty} \|\varphi_n(x)\| \leqslant M.
$$

Take supreme on left side of $\|x\| = 1$, we have $\|\varphi\|_\infty \leqslant M$.

\end{proof}

\section*{Problem 5}

\begin{proof}

If $X$ is a finite dimensional normed space, then we take an orthonormal basis $\{e_1, \dots, e_n\} \subset X$, and linear functionals $\{f_1, \dots, f_n\} \subset X^*$, such that 

$$
f_i (e_j) = \left\{
\begin{aligned}
1 \qquad i = j \\
0 \qquad i \neq j 
\end{aligned}\right.
$$

Hence, for each $x_j$, it can be expressed as $x_j = \sum_{i=1}^n \alpha_i^j e_i$ and $f_k(x_j) = \alpha_k^j$, $\forall k = 1, \dots, n$. Additionally, since $x_j \rightharpoonup x$, we have $f_k(x_j) \rightarrow f_k(x)$, $\forall k$. Hence, 

$$
\|x_j - x\|^2 = \|\sum_{i=1}^n \alpha_i^j e_i -  \sum_{i=1}^n \beta_i e_i\|^2 = \|\sum_{i=1}^n (f_i(x_j) - f_i(x)) e_i \|^2 \leqslant \sum_{i=1}^n |f_i(x_j) - f(x)|^2.
$$

since it is a finite summation and for each $i$, $|f_i(x_j) - f(x)|^2$ goes to $0$, as $j \rightarrow +\infty$. Hence, strongly convergence is proved.

\end{proof}

\section*{Problem 6}
\begin{enumerate}
\item [(i)]
\begin{proof}

$1<p<+\infty$ and $1/p + 1/q = 1$. For any $f\in (\ell^p)^*$, and $x\in \ell^p$, there exists $\alpha = \{\alpha_n\}_{n\in\mathbb N}\in \ell^q$ such that $f(x) = \sum_{i=1}^\infty \alpha_ix_i$.

Hence, $\forall f\in (\ell^p)^*$, $f(e_j) = \sum_{i=1}^\infty \beta_i e_j^i$ and $\sum_{i=1}^\infty |\beta_i|^q < +\infty$.

$$
\|f(e_j) - 0\| = \|\beta_j - 0\| = |\beta_j|.
$$

Since $|\beta_i|^q \rightarrow 0$ as $i \rightarrow +\infty$, we know $\|f(e_j) - 0\| \rightarrow 0$, $\forall f\in (\ell^p)^*$  as $j\rightarrow +\infty$. Hence, $\{e_n\}_{n\geqslant 1}$ weakly converges to $0$ in $\ell^p$.

\end{proof}

\item[(ii)]

\begin{proof}

Any subsequece $\{e_{n_k}\}_{n\geqslant 1}$ is not Cauchy in $\ell^p$ and so it doesn't converge in $\ell^p$. Indeed, for each $k>l$, 

$$
\|e_{n_k} - e_{n_l}\| = \left( \sum_{i = 1}^\infty |e^i_{n_k} - e^i_{n_l}|^p\right)^{1/p} = 2^{1/p}.
$$


\end{proof}
\end{enumerate}


\section*{Problem 7}

\begin{proof}

\begin{enumerate}
\item

$<x,x> = 1/2(\|x+x\|^2 - \|x\|^2 - \|x\|^2) = \|x\|^2 \geqslant 0$. And $<x,x> = 0$ if and only if $x = 0$.

\item 

It is also clear that $<x, y> = <y, x>, \forall x, y \in X$.

\item
We will show $<x, y+z> = <x, y>+<x, z>$, $\forall x, y, z\in X$. By definition, we know

$$
<x, y+z> = \frac{1}{2} (\|x+y+z\|^2 - \|x\|^2 - \|y+z\|^2).
$$
and 
\begin{equation}\label{p7_1}
\begin{aligned}
\|x+y+z\|^2 = & 2\|x\|^2 + 2\|y+z\|^2 - \|x-y-z\|^2 \\
 = & 2\|x+y\|^2 + 2\|z\|^2 - \|x+y-z\|^2
\end{aligned}
\end{equation}

Also, with Parallelogram theorem, we have 

$$
\|x-y-z\|^2 + \|x+y-z\|^2 = 2\|x - z\| + 2\|y\|^2.
$$

Hence, plug it in (\ref{p7_1}) and have 

$$
\|x+y+z\|^2 = \|x\|^2 + \|y+z\|^2 + \|x+y\|^2 + \|z\|^2 - \|x - z\|^2 - \|y\|^2.
$$

which implies

$$
\begin{aligned}
<x, y+z> =& \frac{1}{2} (\|x + y\|^2 - \|x - z\|^2 + \|z\|^2 - \|y\|^2) \\
=& \frac{1}{2} (\|x + y\|^2 - \|y\|^2 - \|x\|^2 - \|x - z\|^2 + \|z\|^2 + \|x\|^2 )\\
 =& <x, y> + <x, z>
\end{aligned}
$$

\item

We need to show that $<\lambda x, y> = \lambda<x, y>$, $\forall x, y\in X, \lambda \in \mathbb R$.

To show this, we need a few steps. Firstly, it holds for $\lambda\in \mathbb N$ and it can be proved by induction. Also, 
$$
\begin{aligned}
<x, -y> =& \frac{1}{2} (\|x - y\|^2  - \|x\|^2 - \|y\|^2) \\
=& \frac{1}{2} (-\|x + y\|^2 + \|y\|^2 + \|x\|^2 )\\
 =& -<x, y> 
\end{aligned}
$$ 

Hence, it holds for $\lambda = -1$ and so holds for $\lambda\in \mathbb Z$. 

Next we will show that it holds for $\lambda \in \mathbb Q$. Let $\lambda = p/q, (q\neq 0), p, q \in \mathbb Z$. Hence, 

$$
q<x, \lambda y> = q <x, \frac{p}{q}y> = <x, py> = p<x, y>.
$$ 

Both sides divided by $q$ and we have $<\lambda x, y> = \lambda<x, y>, \forall \lambda \in \mathbb Q$.

Since $\mathbb Q$ is dense in $\mathbb R$, $\forall \lambda\in\mathbb R$, there exists a sequence of rational numbers $\{\lambda_n\}_{n\in\mathbb N}$ such that $\lambda_n \rightarrow \lambda$. Hence, $<\lambda x, y> = \lambda<x, y>, \forall \lambda \in \mathbb R$.

In conclusion, $<\cdot, \cdot>$ is an inner product.

\end{enumerate}

\end{proof}

\section*{Problem 8}

\begin{enumerate}
\item [(i)]

\begin{proof}

Suppose $\|\cdot\|_1$ is induced by inner product, i.e., $\|\cdot\|_1 = \sqrt{<\cdot, \cdot>}$. However, if so, then $\|\cdot\|$ must satisfy parallelogram identity. For $a = (1,1)^T, b = (-1, 2)^T$, $$
2\|a\|_1^2 + 2\|b\|_1^2 = 26 \neq 18 = \|a - b\|_1^2 + \|a + b\|_1^2.
$$
This is a contradiction.

\end{proof}

\item [(ii)]

Still, it breaks the parallelogram identity.

Let $f(x) = x, g(x) = 2x$. Hence, $\|f\|_\infty = 1, \|g\|_\infty = 2$. But $\|f+g\|_\infty = 3, \|f-g\|_\infty = 1$. So 

$$
\|f+g\|_\infty + \|f-g\|_\infty \neq 2\|f\|_\infty + 2\|g\|_\infty.
$$

\end{enumerate}

\section*{Problem 9}

\begin{proof}

\begin{enumerate}
\item ["$\Rightarrow$"], proved in class. 
 $\left\langle x, x_n \right\rangle$ converges $\left\langle x, x \right\rangle = \|x\|^2$. Hence, 
 
$$
\lim_{n\rightarrow +\infty} \|x_n - x\|^2 = \lim_{n\rightarrow +\infty} \left\langle x_n - x, x_n - x \right\rangle = \lim_{n\rightarrow +\infty} \|x_n\|^2 - 2\left\langle x, x_n \right\rangle + \|x\|^2 = 0
$$

\item ["$\Leftarrow$"]. If $x_n\rightarrow x$, then by Cauchy-Schwartz inequality,

$$
0\leqslant \lim_{n\rightarrow +\infty} \left| \left\langle x_n - x, x \right\rangle\right| \leqslant \lim_{n\rightarrow +\infty} \|x_n - x\| \|x\| = 0.
$$

By squeeze theorem, $\lim_{n\rightarrow +\infty} \left\langle x_n - x, x \right\rangle = 0$. Hence, $x_n \rightharpoonup x$. 

Also, 
$$
\begin{aligned}
0 = \varlimsup_{n\rightarrow +\infty} \|x_n - x\|^2 & = \varlimsup_{n\rightarrow +\infty} \left\langle x_n - x, x_n - x \right\rangle\\
 = &  \varlimsup_{n\rightarrow +\infty} \|x_n\|^2 - 2 \varlimsup_{n\rightarrow +\infty} \left\langle x, x_n \right\rangle + \|x\|^2 \\
= &  \varlimsup_{n\rightarrow +\infty} \|x_n\|^2 - 2 \lim_{n\rightarrow +\infty} \left\langle x, x_n \right\rangle + \|x\|^2 \\
= &  \varlimsup_{n\rightarrow +\infty} \|x_n\|^2 - \|x\|^2
\end{aligned}
$$

Similarly, we have $\varliminf_{n\rightarrow +\infty} \|x_n\|^2 - \|x\|^2 = 0$. Hence, $\lim_{n\rightarrow +\infty} \|x_n\| = \|x\|$.

\end{enumerate}
\end{proof}

\section*{Problem 10}

\begin{proof}

\begin{enumerate}
\item [(i)]

(Shown in class) Since $\{e_n\}_{n\in \mathbb N}$ is an orthonormal basis of $\mathcal H$, for any $x\in \mathcal H$, it can be expressed as

$$
x = \sum_{i=1}^\infty \alpha_i e_i \qquad \alpha_i \in \mathbb R.
$$

Hence, 
$$
\left\langle x, e_i  \right\rangle = \alpha_i \quad \text{and} \quad \left\langle x, x  \right\rangle = \|x\|^2 = \sum_{i=1}^\infty\alpha_i ^2 < +\infty.
$$

Hence, 
$$
\lim_{n\rightarrow +\infty} \left\langle x, e_i  \right\rangle = \lim_{n\rightarrow +\infty} \alpha_i = 0.
$$

i.e., $e_n \rightharpoonup 0$.

\item [(ii)]

Let $\{e_n\}_{n\geqslant1}$ be an orthonormal  basis of $H$ such that $e_n \bot x$, $\forall n\geqslant 2$. Hence, for each $n\in \mathbb N$ and $n\geqslant 2$, let $x_n = x + \lambda e_n (\lambda > 0)$. We want $\|x_n\| = 1$, i.e.,

$$
\|x_n\|^2 = \|x + \lambda e_n\|^2 = \|x\|^2 + \lambda^2 = 1
$$

which yields that $\lambda = \sqrt{1 - \|x\|^2}$. 

Next, we need to show, $x_n = x + \sqrt{1 - \|x\|^2} e_n$ weakly converges to $x$ as $n\rightarrow +\infty$. Indeed, for any arbitrarily taken $y\in H$, use result in (i),

$$
\lim_{n\rightarrow +\infty} \langle y, x_n - x \rangle = \sqrt{1 - \|x\|^2} \langle y, en \rangle = 0
$$

Hence, $x_n \rightharpoonup x$.

\end{enumerate}

\end{proof}



\section*{Problem 11}

\begin{proof}

If $\sum_{n=1}^\infty |\alpha_n|^2 <+\infty $. Let partial sum $S_n = \sum_{i=1}^n \alpha_i v_i$, we need to show that $S_n$ converges as $n\rightarrow +\infty$. Since $H$ is a Hilbert space, it is enough to show $\{S_n\}_{n\geqslant 1}$ is a Cauchy sequence. Indeed, for $m, n \in \mathbb N$, $m > n$, 

$$
\begin{aligned}
\|S_n - S_m\|^2 = \|\sum_{i = n+1}^m \alpha_i v_i\|^2 \leqslant \sum_{i = n+1}^m |\alpha_n|^2.
\end{aligned}
$$

Since $\sum_{n=1}^\infty |\alpha_n|^2 <+\infty $, $\sum_{i = n+1}^m |\alpha_n|^2 \rightarrow 0$ as $m, n\rightarrow +\infty$. Hence, $\{S_n\}$ is Cauchy and so it converges in $H$.

Conversely, if $\{S_n\}$ converges in $H$, and denote the limit as $S$. Hence,  

$$
 +\infty \geqslant \|S\|^2 = \langle \sum_{i = 1}^\infty \alpha_i v_i, \sum_{i = 1}^\infty \alpha_i v_i \rangle = \sum_{n=1}^\infty |\alpha_n|^2.
$$

\end{proof}


\section*{Problem 12}

\begin{enumerate}
\item [(i)]

\begin{proof}

Suppose both $p$ and $q$ are in $\Omega$, such that $p = \pi_\Omega(x), q = \pi_\Omega(x)$. Then, let sequence $\{y_n\}$ be 

$$
y_n = \left\{
\begin{aligned}
p \qquad&  \text{if \ n \ odd}\\
q \qquad&  \text{if \ n \ even}
\end{aligned}\right.
$$

Hence, $\{y_n\}$ converges since $\|y_n - x\|\rightarrow d_\Omega(x)$. And this forces $p = q$.

\end{proof}

\item [(ii)]

To show this, we would like to prove a lemma first.

\begin{lemma}
For any $x, y\in H$, $\alpha > 0$, 
$$
\langle x, y \rangle \leqslant 0 \iff \|x-\alpha y\| \geqslant \|x\|
$$

\end{lemma}

\begin{proof}[Proof of Lemma]

If $\langle x, y \rangle$, $\forall \alpha > 0$, 

$$\langle x-\alpha y, x-\alpha y \rangle = \|x\|^2 + \alpha^2\|y\|^2 - 2\alpha\langle x, y\rangle \geqslant \|x\|^2.
$$

Conversely, if $\|x-\alpha y\| \geqslant \|x\|$, $\forall \alpha > 0$, i.e.,

$$
\langle x-\alpha y, x-\alpha y \rangle = \|x\|^2 + \alpha^2\|y\|^2 - 2\alpha\langle x, y\rangle \geqslant \|x\|^2.
$$

which implies $\alpha^2\|y\|^2 - 2\alpha\langle x, y\rangle \geqslant 0$, and so $\frac{\alpha}{2} \|y\|^2 \geqslant \langle x, y \rangle$. Let $\alpha \rightarrow 0^+$ and obtain $\langle x, y \rangle \leqslant 0$.

\end{proof}

Next we will show the claim. $y = \pi_\Omega (x)$ is equivalent to $\|x - y\| = \min_{w\in\Omega} \|x - w\|$, which is

$$
(\forall w \in \Omega), \|x - y\| \leqslant \|x - w\| = \|x - y - (w - y)\|.
$$

And use the lemma, it is equivalent to $\langle x - y, w - y \rangle \leqslant 0$.

\end{enumerate}


\end{document}